CertifyingDatalog/OrderedGraphValidation.lean
@@ -1,0 +1,268 @@
+import CertifyingDatalog.Basic
+import CertifyingDatalog.Datalog
+import CertifyingDatalog.TreeValidation
+
+
+abbrev orderedProofGraph (τ: signature) [DecidableEq τ.vars] [DecidableEq τ.constants] [DecidableEq τ.relationSymbols] [Inhabited τ.constants] [Hashable τ.constants] [Hashable τ.vars] [Hashable τ.relationSymbols] [ToString τ.constants] [ToString τ.vars] [ToString τ.relationSymbols]:= Array ((groundAtom τ) × List ℕ)
+
+variable {τ: signature} [DecidableEq τ.vars] [DecidableEq τ.constants] [DecidableEq τ.relationSymbols] [Inhabited τ.constants] [Hashable τ.constants] [Hashable τ.vars] [Hashable τ.relationSymbols] [ToString τ.constants] [ToString τ.vars] [ToString τ.relationSymbols]
+
+def labels (proof:orderedProofGraph τ): List (groundAtom τ):= (Array.map Prod.fst proof).toList
+
+lemma labelsMemIffExistsPos (proof:orderedProofGraph τ) (ga: groundAtom τ): ga ∈ labels proof ↔ ∃ (i: ℕ) (h: i < proof.size), Prod.fst (proof[i]) = ga := by
+  unfold labels
+  rw [Array.toList_eq, ← Array.mem_def, Array.mem_iff_get]
+  simp
+
+
+def orderedProofGraph.locallyValid (proof: orderedProofGraph τ) (P: program τ) (d: database τ) (i: ℕ) (hi: i < proof.size):=
+  ∃ (h: ∀ (j: ℕ), j ∈ (Prod.snd proof[i]) → j < i),
+    (Prod.snd proof[i] = [] ∧ d.contains (Prod.fst proof[i]) )
+    ∨ (∃(r: rule τ) (g:grounding τ),
+      r ∈ P ∧
+      ruleGrounding r g =
+      {head:= Prod.fst proof[i], body:=
+      List.map (fun ⟨x, _h⟩ => Prod.fst (Array.get proof (Fin.mk x (Nat.lt_trans (h x _h) hi)))) (Prod.snd proof[i]).attach})
+
+def orderedProofGraph.isValid (proof: orderedProofGraph τ) (P: program τ) (d: database τ): Prop :=
+  ∀ (i: ℕ) (hi: i < proof.size), locallyValid proof P d i hi
+
+lemma isValidSafeAccessSuccessors {proof: orderedProofGraph τ} {P: program τ} {d: database τ} (valid: orderedProofGraph.isValid proof P d) (i: ℕ) (hi: i < proof.size): ∀ (j: ℕ), j ∈ Prod.snd proof[i] → j < proof.size := by
+  simp [orderedProofGraph.isValid, orderedProofGraph.locallyValid] at valid
+  intro j j_mem
+  specialize valid i hi
+  rcases valid with ⟨h,_⟩
+  apply Nat.lt_trans _ hi
+  exact h j j_mem
+
+def checkListSmallerElement (element: ℕ) (l: List ℕ): Except String Unit :=
+  match l with
+  | [] => Except.ok ()
+  | hd::tl => if hd < element
+              then checkListSmallerElement element tl
+              else Except.error "Graph not ordered"
+
+lemma checkListSmallerElementIff (element: ℕ) (l: List ℕ): checkListSmallerElement element l = Except.ok () ↔ ∀ (j: ℕ), j ∈ l → j < element := by
+  induction l with
+  | nil =>
+    simp [checkListSmallerElement]
+  | cons hd tl ih =>
+    simp [checkListSmallerElement]
+    split; simp[*];simp[*]
+
+
+
+
+def validatePosition (m: List τ.relationSymbols → List (rule τ)) (d: database τ) (proof: orderedProofGraph τ) (pos: ℕ) (posValid: pos < proof.size): Except String Unit :=
+  let successors := Prod.snd proof[pos]
+  match h:checkListSmallerElement pos successors with
+  | Except.error e => Except.error e
+  | Except.ok _ =>
+    have hsucc: ∀ (j: ℕ), j ∈ successors → j < pos := by rw [checkListSmallerElementIff] at h; exact h
+
+    if successors.isEmpty
+    then
+      if d.contains (Prod.fst proof[pos]) = true
+      then Except.ok ()
+      else checkRuleMatch m {head:= Prod.fst proof[pos], body := []}
+    else
+      checkRuleMatch m {head:= Prod.fst proof[pos], body:= List.map (fun ⟨x,_h⟩ => Prod.fst (proof.get (Fin.mk x (Nat.lt_trans (hsucc x _h) posValid)))) successors.attach}
+
+
+lemma validatePositionOkIffLocallyValid (P: List (rule τ)) (d: database τ) (proof: orderedProofGraph τ) (pos: ℕ) (posValid: pos < proof.size):
+  validatePosition (parseProgramToSymbolSequenceMap P (fun _ => [])) d proof pos posValid = Except.ok () ↔
+ orderedProofGraph.locallyValid  proof P.toFinset d pos posValid := by
+  simp[orderedProofGraph.locallyValid, validatePosition]
+  split
+  · simp
+    rename_i s checkList
+    have checkList': ¬ checkListSmallerElement pos proof[pos].2 = Except.ok () := by
+      simp[checkList]
+    simp [checkListSmallerElementIff] at checkList'
+    intro h
+    rcases checkList' with ⟨i, i_mem,i_le⟩
+    specialize h i i_mem
+    rw [← not_le] at h
+    contradiction
+
+
+  · rename_i hsuccs
+    rw [checkListSmallerElementIff] at hsuccs
+    split
+    · rename_i succEmpty
+      split
+      · rename_i db_contains
+        simp
+        use hsuccs
+        left
+        simp [← List.isEmpty_iff_eq_nil, succEmpty, db_contains]
+      · rename_i db_contains
+        simp [db_contains, checkRuleMatchOkIffExistsRuleForGroundRule]
+        rw [List.isEmpty_iff_eq_nil] at succEmpty
+        have h: List.attach proof[pos].2 = [] := by
+            simp [succEmpty]
+        rw [h]
+        simp
+        intro _ _ _ _
+        exact hsuccs
+
+    · rename_i succEmpty
+      rw [List.isEmpty_iff_eq_nil] at succEmpty
+      simp [succEmpty, checkRuleMatchOkIffExistsRuleForGroundRule]
+      aesop
+
+
+
+def validateOrderedProof.go (m: List τ.relationSymbols → List (rule τ)) (d: database τ) (proof: orderedProofGraph τ) (pos: ℕ): Except String Unit :=
+  if h: pos < proof.size
+  then
+    match validatePosition m d proof pos h with
+    | Except.error e => Except.error e
+    | Except.ok _ => validateOrderedProof.go m d proof (Nat.succ pos)
+  else
+    Except.ok ()
+termination_by proof.size - pos
+
+
+lemma validateOrderedProofGoSemantics (P: List (rule τ)) (d: database τ) (proof: orderedProofGraph τ) (pos: ℕ):
+validateOrderedProof.go (parseProgramToSymbolSequenceMap P (fun _ => [])) d proof pos = Except.ok () ↔
+∀ (i: ℕ) (h: i < proof.size), pos ≤ i → orderedProofGraph.locallyValid  proof P.toFinset d i h := by
+  induction' h': (proof.size -pos) with n ih generalizing pos
+  · rw [Nat.sub_eq_zero_iff_le, ← not_lt] at h'
+    unfold validateOrderedProof.go
+    simp[h']
+    intro i i_size pos_i
+    exfalso
+    simp at h'
+    have size_i: proof.size ≤ i := Nat.le_trans h' pos_i
+    rw [← not_lt] at size_i
+    contradiction
+  · constructor
+    · intro h i i_size pos_i
+      rw [le_iff_lt_or_eq] at pos_i
+      unfold validateOrderedProof.go at h
+      have pos_size: pos < proof.size := by
+        cases pos_i with
+        | inl pos_i => exact Nat.lt_trans pos_i i_size
+        | inr pos_i => rw [pos_i]; exact i_size
+      simp [pos_size] at h
+      split at h
+      · simp at h
+      · rename_i validatePos
+        rw [validatePositionOkIffLocallyValid] at validatePos
+        cases pos_i with
+        | inl pos_i =>
+          have size_pos: Array.size proof - Nat.succ pos = n := by
+            rw [Nat.sub_succ, h', Nat.pred_succ]
+          specialize ih (Nat.succ pos) size_pos
+          rw [ih] at h
+          apply h
+          apply Nat.succ_le_of_lt
+          exact pos_i
+        | inr pos_i =>
+          simp_rw [← pos_i]
+          exact validatePos
+    · intro h
+      unfold validateOrderedProof.go
+      split
+      · rename_i pos_size
+        split
+        · rename_i s validatePos
+          have validatePos': ¬ validatePosition (parseProgramToSymbolSequenceMap P fun _ => []) d proof pos pos_size = Except.ok () := by simp [validatePos]
+          rw [validatePositionOkIffLocallyValid] at validatePos'
+          specialize h pos pos_size
+          simp at h
+          contradiction
+        · have size_pos: Array.size proof - Nat.succ pos = n := by
+            rw [Nat.sub_succ, h', Nat.pred_succ]
+          specialize ih (Nat.succ pos) size_pos
+          rw [ih]
+          intro i i_proof pos_i
+          apply h
+          rw [Nat.succ_le] at pos_i
+          apply Nat.le_of_lt pos_i
+      · rfl
+
+
+
+def validateOrderedProof (m: List τ.relationSymbols → List (rule τ)) (d: database τ) (proof: orderedProofGraph τ): Except String Unit := validateOrderedProof.go m d proof 0
+
+lemma validateOrderedProofSemantics(P: List (rule τ)) (d: database τ) (proof: orderedProofGraph τ):
+validateOrderedProof (parseProgramToSymbolSequenceMap P (fun _ => [])) d proof = Except.ok () ↔ orderedProofGraph.isValid proof P.toFinset d := by
+  simp [validateOrderedProof, orderedProofGraph.isValid, validateOrderedProofGoSemantics]
+
+def extractProofTree (proof: orderedProofGraph τ) {P: program τ} {d: database τ} (valid: orderedProofGraph.isValid proof P d) (pos: ℕ) (posValid: pos < proof.size): proofTree τ :=
+  tree.node proof[pos].1 (List.map (fun ⟨x, _h⟩ => extractProofTree proof valid x (isValidSafeAccessSuccessors valid pos posValid x _h)) proof[pos].2.attach)
+termination_by pos
+decreasing_by
+  simp_wf
+  simp [orderedProofGraph.isValid, orderedProofGraph.locallyValid] at valid
+  specialize valid pos posValid
+  rcases valid with ⟨h,_⟩
+  exact h x _h
+
+lemma extractProofTreeRoot (proof: orderedProofGraph τ) {P: program τ} {d: database τ} (valid: orderedProofGraph.isValid proof P d) (pos: ℕ) (posValid: pos < proof.size):  root (extractProofTree proof valid pos posValid) = proof[pos].1 := by
+  unfold extractProofTree
+  unfold root
+  simp
+
+lemma extractProofTreeIsValid (proof: orderedProofGraph τ) {P: program τ} {d: database τ} (valid: orderedProofGraph.isValid proof P d) (pos: ℕ) (posValid: pos < proof.size): isValid P d (extractProofTree proof valid pos posValid) := by
+  induction' pos using Nat.strongInductionOn with pos ih
+  simp [orderedProofGraph.isValid, orderedProofGraph.locallyValid] at valid
+  specialize valid pos posValid
+  rcases valid with ⟨h, h'⟩
+  cases h' with
+  | inl h' =>
+    unfold extractProofTree
+    rcases h' with ⟨succEmpty, dbContain⟩
+    have attachEmpty: List.attach proof[pos].2 = [] := by
+      simp [succEmpty]
+    simp [attachEmpty]
+    unfold isValid
+    right
+    simp [dbContain]
+  | inr h' =>
+    unfold extractProofTree
+    unfold isValid
+    left
+    rcases h' with ⟨r, rP, g, ground⟩
+    use r
+    use g
+    simp [rP]
+    constructor
+    · rw [ground, groundRuleEquality]
+      constructor
+      · simp
+      · apply List.ext_get
+        simp
+
+        intro n h1 h2
+        simp
+        rw [extractProofTreeRoot]
+    · rw [List.forall_iff_forall_mem]
+      simp
+      intro t x x_mem ht
+      rw [← ht]
+      apply ih
+      apply h
+      exact x_mem
+
+theorem validateOrderedProofIffValidAndSubset (P: List (rule τ)) (d: database τ) (proof: orderedProofGraph τ):
+validateOrderedProof (parseProgramToSymbolSequenceMap P (fun _ => [])) d proof = Except.ok () ↔ orderedProofGraph.isValid proof P.toFinset d ∧ (labels proof).toSet ⊆ proofTheoreticSemantics P.toFinset d := by
+  constructor
+  intro h
+  rw [validateOrderedProofSemantics] at h
+  simp [h]
+  simp [proofTheoreticSemantics, Set.subset_def, ← List.toSet_mem]
+  intro ga ga_mem
+  rw [labelsMemIffExistsPos] at ga_mem
+  rcases ga_mem with ⟨pos, pos_valid, get_pos⟩
+  use extractProofTree proof h pos pos_valid
+  constructor
+  · simp [extractProofTreeRoot, get_pos]
+  · apply extractProofTreeIsValid
+
+  intro h
+  rcases h with ⟨h, _⟩
+  rw [validateOrderedProofSemantics]
+  exact h
